src/Std/Data/DTreeMap/Internal/Queries.lean
@@ -5,6 +5,7 @@ Authors: Markus Himmel
 -/
 prelude
 import Std.Data.DTreeMap.Internal.Def
+import Std.Data.DTreeMap.Internal.Balanced
 import Std.Classes.Ord
 
 /-!
@@ -21,15 +22,6 @@ universe u v w
 variable {α : Type u} {β : α → Type v} {γ : α → Type w} {δ : Type w} {m : Type w → Type w}
 
 namespace Std.DTreeMap.Internal.Impl
-
-/-- The size information stored in the tree. -/
-@[inline]
-def size : Impl α β → Nat
-  | inner sz _ _ _ _ => sz
-  | leaf => 0
-
-@[Std.Internal.tree_tac] theorem size_leaf : (Impl.leaf : Impl α β).size = 0 := rfl
-@[Std.Internal.tree_tac] theorem size_inner {sz k v l r} : (Impl.inner sz k v l r : Impl α β).size = sz := rfl
 
 /-- Returns `true` if the given key is contained in the map. -/
 def contains [Ord α] (k : α) (t : Impl α β) : Bool :=
@@ -216,6 +208,246 @@ variable {β : Type v}
 /-- Returns a `List` of the key/value pairs in order. -/
 @[inline] def toArray (t : Impl α (fun _ => β)) : Array (α × β) :=
   t.foldl (init := #[]) fun l k v => l.push (k, v)
+
+end Const
+
+/-- The smallest element of `t`. -/
+def min? [Ord α] : Impl α β → Option ((a : α) × β a)
+  | .leaf => none
+  | .inner _ k v .leaf _ => some ⟨k, v⟩
+  | .inner _ _ _ l@(.inner _ _ _ _ _) _ => l.min?
+
+/-- The smallest element of `t`. -/
+def min [Ord α] : (t : Impl α β) → (htb : t.Balanced) → (h : t.isEmpty = false) → (a : α) × β a
+  | .leaf, h => False.elim <| sorry
+  | .inner _ k v .leaf _, _ => ⟨k, v⟩
+  | .inner _ _ _ l@(.inner _ _ _ _ _) _, _ => l.min?
+
+/-- The smallest element of `t`. Panics if the map is empty. -/
+def min! [Ord α] [Inhabited ((a : α) × β a)] : Impl α β → (a : α) × β a
+  | .leaf => panic "Map is empty"
+  | .inner _ k v .leaf _ => ⟨k, v⟩
+  | .inner _ _ _ l@(.inner _ _ _ _ _) _ => l.min!
+
+/-- The largest element of `t`. -/
+def max? [Ord α] : Impl α β → Option ((a : α) × β a)
+  | .leaf => none
+  | .inner _ k v _ .leaf => some ⟨k, v⟩
+  | .inner _ _ _ _ r@(.inner _ _ _ _ _) => r.max?
+
+/-- The largest element of `t`. -/
+def max [Ord α] : (t : Impl α β) → (h : t.isEmpty = false) → (a : α) × β a
+  | .leaf, h => False.elim <| Bool.true_eq_false ▸ h
+  | .inner _ k v _ .leaf => some ⟨k, v⟩
+  | .inner _ _ _ _ r@(.inner _ _ _ _ _) => r.max?
+
+/-- The largest element of `t`. Panics if the map is empty. -/
+def max! [Ord α] [Inhabited ((a : α) × β a)] : Impl α β → (a : α) × β a
+  | .leaf => panic "Map is empty"
+  | .inner _ k v _ .leaf => ⟨k, v⟩
+  | .inner _ _ _ _ r@(.inner _ _ _ _ _) => r.max!
+
+/-- The smallest key of `t`. -/
+def minKey? [Ord α] : Impl α β → Option α
+  | .leaf => none
+  | .inner _ k _ .leaf _ => some k
+  | .inner _ _ _ l@(.inner _ _ _ _ _) _ => minKey? l
+
+/-- The largest key of `t`. -/
+def maxKey? [Ord α] : Impl α β → Option α
+  | .leaf => none
+  | .inner _ k _ _ .leaf => some k
+  | .inner _ _ _ _ r@(.inner _ _ _ _ _) => maxKey? r
+
+/-- The smallest key of `t`. Panics if the map is empty. -/
+def minKey! [Ord α] [Inhabited α] : Impl α β → α
+  | .leaf => panic "Map is empty"
+  | .inner _ k _ .leaf _ => k
+  | .inner _ _ _ l@(.inner _ _ _ _ _) _ => minKey! l
+
+/-- The largest key of `t`. Panics if the map is empty. -/
+def maxKey! [Ord α] [Inhabited α] : Impl α β → α
+  | .leaf => panic "Map is empty"
+  | .inner _ k _ _ .leaf => k
+  | .inner _ _ _ _ r@(.inner _ _ _ _ _) => maxKey! r
+
+/-- The smallest element of `t` that is not less than `k`. Also known as `lookupGE` or `ceil`. -/
+@[inline]
+def getEntryGE? [Ord α] (k : α) : Impl α β → Option ((a : α) × β a) :=
+  go none
+where
+  go (best : Option ((a : α) × β a)) : Impl α β → Option ((a : α) × β a)
+  | .leaf => best
+  | .inner _ ky y l r => match compare k ky with
+    | .lt => go (some ⟨ky, y⟩) l
+    | .eq => some ⟨ky, y⟩
+    | .gt => go best r
+
+/-- The smallest element of `t` that is greater than `k`. Also known as `lookupGT` or `higher`. -/
+@[inline]
+def getEntryGT? [Ord α] (k : α) : Impl α β → Option ((a : α) × β a) :=
+  go none
+where
+  go (best : Option ((a : α) × β a)) : Impl α β → Option ((a : α) × β a)
+  | .leaf => best
+  | .inner _ ky y l r => match compare k ky with
+    | .lt => go (some ⟨ky, y⟩) l
+    | _ => go best r
+
+/-- The largest element of `t` that is not greater than `k`. Also known as `floor`. -/
+@[inline]
+def getEntryLE? [Ord α] (k : α) : Impl α β → Option ((a : α) × β a) :=
+  go none
+where
+  go (best : Option ((a : α) × β a)) : Impl α β → Option ((a : α) × β a)
+  | .leaf => best
+  | .inner _ ky y l r => match compare k ky with
+    | .lt => go best l
+    | .eq => some ⟨ky, y⟩
+    | .gt => go (some ⟨ky, y⟩) r
+
+/-- The largest element of `t` that is less than `k`. Also known as `lower`. -/
+@[inline]
+def getEntryLT? [Ord α] (k : α) : Impl α β → Option ((a : α) × β a) :=
+  go none
+where
+  go (best : Option ((a : α) × β a)) : Impl α β → Option ((a : α) × β a)
+  | .leaf => best
+  | .inner _ ky y l r => match compare k ky with
+    | .gt => go (some ⟨ky, y⟩) r
+    | _ => go best l
+
+/-- The smallest key of `t` that is not less than `k`. Also known as `lookupGE` or `ceil`. -/
+@[inline]
+def getKeyGE? [Ord α] (k : α) : Impl α β → Option α :=
+  go none
+where
+  go (best : Option α) : Impl α β → Option α
+  | .leaf => best
+  | .inner _ ky _ l r => match compare k ky with
+    | .lt => go (some ky) l
+    | .eq => some ky
+    | .gt => go best r
+
+/-- The smallest key of `t` that is greater than `k`. Also known as `lookupGT` or `higher`. -/
+@[inline]
+def getKeyGT? [Ord α] (k : α) : Impl α β → Option α :=
+  go none
+where
+  go (best : Option α) : Impl α β → Option α
+  | .leaf => best
+  | .inner _ ky _ l r => match compare k ky with
+    | .lt => go (some ky) l
+    | _ => go best r
+
+/-- The largest key of `t` that is not greater than `k`. Also known as `floor`. -/
+@[inline]
+def getKeyLE? [Ord α] (k : α) : Impl α β → Option α :=
+  go none
+where
+  go (best : Option α) : Impl α β → Option α
+  | .leaf => best
+  | .inner _ ky y l r => match compare k ky with
+    | .lt => go best l
+    | .eq => some ky
+    | .gt => go (some ky) r
+
+/-- The largest key of `t` that is less than `k`. Also known as `lower`. -/
+@[inline]
+def getKeyLT? [Ord α] (k : α) : Impl α β → Option α :=
+  go none
+where
+  go (best : Option α) : Impl α β → Option α
+  | .leaf => best
+  | .inner _ ky y l r => match compare k ky with
+    | .gt => go (some ky) r
+    | _ => go best l
+
+namespace Const
+
+variable {β : Type v}
+
+/-- The smallest element of `t`. -/
+def min? [Ord α] : Impl α (fun _ => β) → Option (α × β)
+  | .leaf => none
+  | .inner _ k v .leaf _ => some ⟨k, v⟩
+  | .inner _ _ _ l@(.inner _ _ _ _ _) _ => min? l
+
+/-- The largest element of `t`. -/
+def max? [Ord α] : Impl α (fun _ => β) → Option (α × β)
+  | .leaf => none
+  | .inner _ k v _ .leaf => some ⟨k, v⟩
+  | .inner _ _ _ _ r@(.inner _ _ _ _ _) => max? r
+
+/-- The smallest element of `t`. Panics if the map is empty. -/
+def min! [Ord α] [Inhabited α] [Inhabited β] : Impl α (fun _ => β) → α × β
+  | .leaf => letI : Inhabited (α × β) := ⟨⟨default, default⟩⟩; panic "Map is empty"
+  | .inner _ k v .leaf _ => ⟨k, v⟩
+  | .inner _ _ _ l@(.inner _ _ _ _ _) _ => min! l
+
+/-- The largest element of `t`. Panics if the map is empty. -/
+def max! [Ord α] [Inhabited α] [Inhabited β] : Impl α (fun _ => β) → α × β
+  | .leaf => letI : Inhabited (α × β) := ⟨⟨default, default⟩⟩; panic "Map is empty"
+  | .inner _ k v _ .leaf => ⟨k, v⟩
+  | .inner _ _ _ _ r@(.inner _ _ _ _ _) => max! r
+
+/-- The smallest element of `t`. Panics if the map is empty. -/
+def min! [Ord α] [Inhabited α] [Inhabited β] : Impl α (fun _ => β) → α × β
+  | .leaf => letI : Inhabited (α × β) := ⟨⟨default, default⟩⟩; panic "Map is empty"
+  | .inner _ k v .leaf _ => ⟨k, v⟩
+  | .inner _ _ _ l@(.inner _ _ _ _ _) _ => min! l
+
+/-- The largest element of `t`. Panics if the map is empty. -/
+def max! [Ord α] [Inhabited α] [Inhabited β] : Impl α (fun _ => β) → α × β
+  | .leaf => letI : Inhabited (α × β) := ⟨⟨default, default⟩⟩; panic "Map is empty"
+  | .inner _ k v _ .leaf => ⟨k, v⟩
+  | .inner _ _ _ _ r@(.inner _ _ _ _ _) => max! r
+
+/-- The smallest element of `t` that is not less than `k`. Also known as `lookupGE` or `ceil`. -/
+@[inline]
+def getEntryGE? [Ord α] (k : α) : Impl α (fun _ => β) → Option (α × β) :=
+  go none
+where
+  go (best : Option (α × β)) : Impl α (fun _ => β) → Option (α × β)
+  | .leaf => best
+  | .inner _ ky y l r => match compare k ky with
+    | .lt => go (some ⟨ky, y⟩) l
+    | .eq => some ⟨ky, y⟩
+    | .gt => go best r
+
+/-- The smallest element of `t` that is greater than `k`. Also known as `lookupGT` or `higher`. -/
+@[inline]
+def getEntryGT? [Ord α] (k : α) : Impl α (fun _ => β) → Option (α × β) :=
+  go none
+where
+  go (best : Option (α × β)) : Impl α (fun _ => β) → Option (α × β)
+  | .leaf => best
+  | .inner _ ky y l r => match compare k ky with
+    | .lt => go (some ⟨ky, y⟩) l
+    | _ => go best r
+
+/-- The largest element of `t` that is not greater than `k`. Also known as `floor`. -/
+@[inline]
+def getEntryLE? [Ord α] (k : α) : Impl α (fun _ => β) → Option (α × β) :=
+  go none
+where
+  go (best : Option (α × β)) : Impl α (fun _ => β) → Option (α × β)
+  | .leaf => best
+  | .inner _ ky y l r => match compare k ky with
+    | .lt => go best l
+    | .eq => some ⟨ky, y⟩
+    | .gt => go (some ⟨ky, y⟩) r
+
+/-- The largest element of `t` that is less than `k`. Also known as `lower`. -/
+@[inline]
+def getEntryLT? [Ord α] (k : α) : Impl α (fun _ => β) → Option (α × β) :=
+  go none
+where
+  go (best : Option (α × β)) : Impl α (fun _ => β) → Option (α × β)
+  | .leaf => best
+  | .inner _ ky y l r => match compare k ky with
+    | .gt => go (some ⟨ky, y⟩) r
+    | _ => go best l
 
 end Const
 
