src/Std/Data/DTreeMap/Internal/Balanced.lean
@@ -1,0 +1,56 @@
+/-
+Copyright (c) 2024 Lean FRO, LLC. All rights reserved.
+Released under Apache 2.0 license as described in the file LICENSE.
+Authors: Markus Himmel
+-/
+prelude
+import Init.Data.AC
+import Std.Data.DTreeMap.Internal.Def
+
+/-!
+# `Balanced` predicate
+
+This file defines what it means for a tree map to be balanced. This definition is encoded in the
+`Balanced` predicate.
+-/
+
+set_option autoImplicit false
+set_option linter.all true
+
+universe u v w
+
+variable {α : Type u} {β : α → Type v}
+
+namespace Std.DTreeMap.Internal.Impl
+
+/--
+Predicate for local balance at a node of the tree. We don't provide API for this, preferring
+instead to use automation to dispatch goals about balance.
+-/
+@[Std.Internal.tree_tac]
+def BalancedAtRoot (left right : Nat) : Prop :=
+  left + right ≤ 1 ∨ (left ≤ delta * right ∧ right ≤ delta * left)
+
+/--
+Predicate that states that the stored size information in a tree is correct and that it is
+balanced.
+-/
+inductive Balanced : Impl α β → Prop where
+  /-- Leaf is balanced. -/
+  | leaf : Balanced leaf
+  /--
+  Inner node is balanced if it is locally balanced, both children are balanced and size
+  information is correct.
+  -/
+  | inner {sz k v l r} : Balanced l → Balanced r →
+      BalancedAtRoot l.size r.size → sz = l.size + 1 + r.size → Balanced (inner sz k v l r)
+
+attribute [Std.Internal.tree_tac] Balanced.leaf
+
+@[Std.Internal.tree_tac]
+theorem balanced_inner_iff {sz k v l r} : Balanced (Impl.inner sz k v l r : Impl α β) ↔
+    Balanced l ∧ Balanced r ∧ BalancedAtRoot l.size r.size ∧ sz = l.size + 1 + r.size :=
+  ⟨by rintro (_|⟨h₁, h₂, h₃, h₄⟩); exact ⟨h₁, h₂, h₃, h₄⟩,
+   fun ⟨h₁, h₂, h₃, h₄⟩ => .inner h₁ h₂ h₃ h₄⟩
+
+end Std.DTreeMap.Internal.Impl
